wip

Kraken/Examples/Examples.lean
@@ -662,8 +662,8 @@ def klog : DSimproc := fun e => do
   -- We log every top-level term get a trace of the various states of the dsimp
   -- call.
   let s := (← get).numSteps
-  if s = 789 then
-    return .rfl (done := true)
+  /- if s = 789 then -/
+  /-   return .rfl (done := true) -/
   if e.isApp && e.getAppFn'.isConstOf ``Effects.All then
     logInfo m!"klog: step {s} visiting\n{e}"
   return .rfl
@@ -706,14 +706,17 @@ def kdsimpProj : DSimproc := fun e => do
   reduceProjCont? (← unfoldDefinition? e)
 
 def kLiftLets : DSimproc := fun e => do
-  let (es, st) ← Meta.ExtractLets.extract #[e] |>.run { onlyGivenNames := true } |>.run' {} |>.run { givenNames := [] }
-  unless st.decls.size != 0 do return .rfl
+  -- We only lift lets to the top-level (which is always an application of
+  -- Effects.all)
+  unless e.isApp && e.getAppFn'.isConstOf ``Effects.All do return .rfl
+
+  let (es, st) ← ExtractLets.extract #[e] |>.run {} |>.run' {} |>.run { givenNames := [] }
+  unless st.decls.size > 0 do return .rfl
+
   let e' := Meta.ExtractLets.mkLetDecls st.decls es[0]!
-  if isSameExpr e e' then
-    return .rfl
-  else
-    let e' ← Sym.share e'
-    return .step e'
+  let e' ← Sym.share e'
+  /- logInfo m!"liftLets produces {e'}" -/
+  return .step e'
 
 -- TODO: make our tactic take an optional config to aid debugging
 @[grind_tactic symKStep]
@@ -739,7 +742,7 @@ def evalSymKStep : Grind.GrindTactic :=
 
   let goal ← Grind.liftGrindM (Sym.dsimp
     (config := { maxSteps := 1000000 })
-    (methods := { pre := klog >> kLiftLets >> kdeltaBetaOnly decls >> kdsimpMatch >> kdsimpProj >> kbeta})
+    (methods := { pre := /-klog >> -/kLiftLets >> kdeltaBetaOnly decls >> kdsimpMatch >> kdsimpProj >> kbeta})
     goal)
 
   let mvarId ← mvarId.replaceTargetDefEq goal
@@ -788,38 +791,36 @@ example [layout : Layout] s : Step1 (layout p5) (s, layout.start) (fun s => s.1.
   sym => 
   kstep
   tactic =>
-  lift_lets
-  sym =>
-  kstep
-  sorry
+  intros
+  decide
 
   /- tactic => -/
   /- lift_lets -/
   /- dsimp (zeta:=false)(beta:=true)(eta:=false)(iota:=true)(proj:=true) only [Effects.All] -/
 
-/- def bigp := parseFile("./ecc-secp521r1-modp.S") -/
+def bigp := parseFile("./ecc-secp521r1-modp.S")
 
-/- set_option maxRecDepth 4000 -/
-/- set_option maxHeartbeats 2000000 -/
+set_option maxRecDepth 4000
+set_option maxHeartbeats 2000000
 
-/- example [layout : Layout] s : Step1 (layout bigp) (s, layout.start) (fun s => s.1.regs.rax = 0) := by -/
-/-   -- Refine the state to make registers apparent -- note that `cases` consumes -/
-/-   -- the hypothesis, and substitutes it, so we make a copy of it to have a -/
-/-   -- refined state in the hypotheses, not the goal. -/
-/-   let ss := s -/
-/-   change (Step1 _ (ss, _) _) -/
-/-   cases s with | mk regs flags mem => -/
-/-   cases regs with | mk rax => -/
-/-   -- Rewrite the program to make layout, addresses, etc. apparent -/
-/-   delta bigp -/
-/-   dsimp only [Step1,Executable.straightline] -/
-/-   rw [Executable.directivesFromStart] -/
-/-   simp [List.mapIdx,List.mapIdx.go] -/
-/-   sym => -/ 
-/-   kstep -/
-/-   sorry -/
-/-   tactic => -/
-/-   lift_lets -/
-/-   revert -/
-/-   sorry -/
+example [layout : Layout] s : Step1 (layout bigp) (s, layout.start) (fun s => s.1.regs.rax = 0) := by
+  -- Refine the state to make registers apparent -- note that `cases` consumes
+  -- the hypothesis, and substitutes it, so we make a copy of it to have a
+  -- refined state in the hypotheses, not the goal.
+  let ss := s
+  change (Step1 _ (ss, _) _)
+  cases s with | mk regs flags mem =>
+  cases regs with | mk rax =>
+  -- Rewrite the program to make layout, addresses, etc. apparent
+  delta bigp
+  dsimp only [Step1,Executable.straightline]
+  rw [Executable.directivesFromStart]
+  simp [List.mapIdx,List.mapIdx.go]
+  sym => 
+  kstep
+  sorry
+  tactic =>
+  lift_lets
+  revert
+  sorry
 
